raw_init_+ raw_learned_clss ~> raw_ + learned_clss
The aim of this change is to improve reusability by better
abstraction. Instead of having two 'clss in the 2-WL, we use only
one and have a criterion whteher a clause is learned or not. This also
means less operations on the 'clss

This will ease the move to iterators instead of objects that are
convertible to multiset like lists.

Weidenbach_Book/CDCL_Two_Watched_Literals.thy
@@ -63,11 +63,14 @@ lemma clause_def_lambda:
   "clause = (\<lambda>C. mset (raw_clause C))"
   by (auto simp: clause_def)
 
-abbreviation raw_clss :: "'v twl_state \<Rightarrow> 'v clauses" where
-  "raw_clss S \<equiv> mset (map clause (raw_init_clss S @ raw_learned_clss S))"
-
-abbreviation raw_clss_l :: "'a twl_clause list \<Rightarrow> 'a literal multiset multiset" where
+abbreviation raw_clss_l :: "'a twl_clause list \<Rightarrow> 'a clauses" where
   "raw_clss_l C \<equiv> mset (map clause C)"
+
+abbreviation raw_clauses :: "'v twl_state \<Rightarrow> 'v twl_clause list" where
+  "raw_clauses S \<equiv> raw_init_clss S @ raw_learned_clss S"
+
+abbreviation raw_clss :: "'v twl_state \<Rightarrow> 'v clauses" where
+  "raw_clss S \<equiv> raw_clss_l (raw_clauses S)"
 
 interpretation raw_cls clause .
 
@@ -97,6 +100,9 @@ proof -
   then show ?thesis by fast
 qed
 
+abbreviation conc_learned_clss where
+"conc_learned_clss \<equiv> \<lambda>S. mset (map clause (raw_learned_clss S))"
+
 interpretation twl: abs_state\<^sub>W_ops
   clause
   raw_clss_l "op @"
@@ -106,7 +112,8 @@ interpretation twl: abs_state\<^sub>W_ops
 
   raw_clause "\<lambda>C. TWL_Clause [] C"
   trail "\<lambda>S. hd (raw_trail S)"
-  raw_init_clss raw_learned_clss backtrack_lvl raw_conflicting
+  "(\<lambda>S. raw_init_clss S @ raw_learned_clss S)" backtrack_lvl raw_conflicting
+  conc_learned_clss
   rewrites
     "twl.mmset_of_mlit = mmset_of_mlit"
 proof goal_cases
@@ -132,13 +139,13 @@ definition
 where
   "candidates_propagate S =
    {(L, C) | L C.
-     C \<in> set (twl.raw_clauses S)  \<and>
+     C \<in> set (raw_clauses S)  \<and>
      set (watched C) - (uminus ` lits_of_l (trail S)) = {L} \<and>
      undefined_lit (raw_trail S) L}"
 
 definition candidates_conflict :: "'v twl_state \<Rightarrow> 'v twl_clause set" where
   "candidates_conflict S =
-   {C. C \<in> set (twl.raw_clauses S) \<and>
+   {C. C \<in> set (raw_clauses S) \<and>
      set (watched C) \<subseteq> uminus ` lits_of_l (raw_trail S)}"
 
 primrec (nonexhaustive) index :: "'a list \<Rightarrow>'a \<Rightarrow> nat" where
@@ -259,7 +266,7 @@ lemma wf_twl_cls_append:
 
 definition wf_twl_state :: "'v twl_state \<Rightarrow> bool" where
   "wf_twl_state S \<longleftrightarrow>
-    (\<forall>C \<in> set (twl.raw_clauses S). wf_twl_cls (raw_trail S) C) \<and> no_dup (raw_trail S)"
+    (\<forall>C \<in> set (raw_clauses S). wf_twl_cls (raw_trail S) C) \<and> no_dup (raw_trail S)"
 
 lemma wf_candidates_propagate_sound:
   assumes wf: "wf_twl_state S" and
@@ -277,7 +284,7 @@ proof
     "C \<in> set (N @ U)"
     "set (watched C) - uminus ` lits_of_l M = {L}"
     "undefined_lit M L"
-    using cand unfolding candidates_propagate_def MNU_defs twl.raw_clauses_def by auto
+    using cand unfolding candidates_propagate_def MNU_defs by auto
 
   obtain W UW where cw_eq: "C = TWL_Clause W UW"
     by (cases C)
@@ -286,7 +293,7 @@ proof
     using cw(2) cw_eq by auto
 
   have wf_c: "wf_twl_cls M C"
-    using wf cw(1) unfolding wf_twl_state_def by (simp add: twl.raw_clauses_def)
+    using wf cw(1) unfolding wf_twl_state_def by simp
 
   have w_nw:
     "distinct W"
@@ -361,7 +368,7 @@ qed
 
 lemma wf_candidates_propagate_complete:
   assumes wf: "wf_twl_state S" and
-    c_mem: "C \<in> set (twl.raw_clauses S)" and
+    c_mem: "C \<in> set (raw_clauses S)" and
     l_mem: "L \<in> set (raw_clause C)" and
     unsat: "trail S \<Turnstile>as CNot (mset_set (set (raw_clause C) - {L}))" and
     undef: "undefined_lit (raw_trail S) L"
@@ -445,7 +452,7 @@ qed
 lemma wf_candidates_conflict_sound:
   assumes wf: "wf_twl_state S" and
     cand: "C \<in> candidates_conflict S"
-  shows "trail S \<Turnstile>as CNot (clause C) \<and> C \<in> set (twl.raw_clauses S)"
+  shows "trail S \<Turnstile>as CNot (clause C) \<and> C \<in> set (raw_clauses S)"
 proof
   def M \<equiv> "raw_trail S"
   def N \<equiv> "raw_init_clss S"
@@ -456,13 +463,13 @@ proof
   have cw:
     "C \<in> set (N @ U)"
     "set (watched C) \<subseteq> uminus ` lits_of_l (trail S)"
-    using cand[unfolded candidates_conflict_def, simplified] unfolding twl.raw_clauses_def by auto
+    using cand[unfolded candidates_conflict_def, simplified] by auto
 
   obtain W UW where cw_eq: "C = TWL_Clause W UW"
     by (cases C, blast)
 
   have wf_c: "wf_twl_cls M C"
-    using wf cw(1) unfolding wf_twl_state_def by (simp add: comp_def twl.raw_clauses_def)
+    using wf cw(1) unfolding wf_twl_state_def by simp
 
   have w_nw:
     "distinct W"
@@ -501,19 +508,19 @@ proof
   then show "trail S \<Turnstile>as CNot (clause C)"
     unfolding CNot_def true_annots_def clause_def by auto
 
-  show "C \<in> set (twl.raw_clauses S)"
-    using cw unfolding twl.raw_clauses_def by auto
+  show "C \<in> set (raw_clauses S)"
+    using cw by auto
 qed
 
 lemma wf_candidates_conflict_complete:
   assumes wf: "wf_twl_state S" and
-    c_mem: "C \<in> set (twl.raw_clauses S)" and
+    c_mem: "C \<in> set (raw_clauses S)" and
     unsat: "trail S \<Turnstile>as CNot (clause C)"
   shows "C \<in> candidates_conflict S"
 proof -
   def M \<equiv> "raw_trail S"
   def N \<equiv> "twl.conc_init_clss S"
-  def U \<equiv> "twl.conc_learned_clss S"
+  def U \<equiv> "conc_learned_clss S"
 
   note MNU_defs [simp] = M_def N_def U_def
 
@@ -550,7 +557,7 @@ morphisms rough_state_of_twl twl_of_rough_state
 proof -
   have "TWL_State ([]::('v, 'v twl_clause) ann_lits)
     [] [] 0 None \<in> {S:: 'v twl_state. wf_twl_state S} "
-    by (auto simp: wf_twl_state_def twl.raw_clauses_def)
+    by (auto simp: wf_twl_state_def)
   then show ?thesis by auto
 qed
 
@@ -574,13 +581,16 @@ abbreviation trail_twl :: "'a wf_twl \<Rightarrow> ('a, 'a literal multiset) ann
 "trail_twl S \<equiv> trail (rough_state_of_twl S)"
 
 abbreviation raw_clauses_twl :: "'a wf_twl \<Rightarrow> 'a twl_clause list" where
-"raw_clauses_twl S \<equiv> twl.raw_clauses (rough_state_of_twl S)"
+"raw_clauses_twl S \<equiv> raw_clauses (rough_state_of_twl S)"
 
 abbreviation raw_init_clss_twl :: "'a wf_twl \<Rightarrow> 'a twl_clause list" where
 "raw_init_clss_twl S \<equiv> raw_init_clss (rough_state_of_twl S)"
 
 abbreviation raw_learned_clss_twl :: "'a wf_twl \<Rightarrow> 'a twl_clause list" where
 "raw_learned_clss_twl S \<equiv> raw_learned_clss (rough_state_of_twl S)"
+
+abbreviation conc_learned_clss_twl :: "'a wf_twl \<Rightarrow> 'a clauses" where
+"conc_learned_clss_twl S \<equiv> conc_learned_clss (rough_state_of_twl S)"
 
 abbreviation backtrack_lvl_twl where
 "backtrack_lvl_twl S \<equiv> backtrack_lvl (rough_state_of_twl S)"
@@ -676,6 +686,10 @@ lemma unchanged_init_state[simp]:
   "backtrack_lvl (init_state N) = 0"
   "raw_conflicting (init_state N) = None"
   unfolding init_state_def by (rule unchanged_fold_add_init_cls)+
+
+lemma conc_init_clss[simp]:
+  "twl.conc_init_clss (TWL_State M N U k C) = raw_clss_l N"
+  by (simp add: twl.conc_init_clss_def)
 
 lemma clauses_init_fold_add_init:
   "no_dup M \<Longrightarrow>
