Weidenbach_Book/CDCL_Two_Watched_Literals_Invariant.thy
@@ -23,10 +23,13 @@ lemma mset_map_removeAll_cond:
   = mset (removeAll (clause C) (map clause N))"
   by (induction N) auto
 
+lemma raw_clss_l_raw_init_clss_conc_init_clss[simp]:
+  "raw_clss_l (raw_init_clss S) = twl.conc_init_clss S"
+  by (cases S) auto
 lemma mset_raw_init_clss_init_state:
-  "mset (map clause (raw_init_clss (init_state (map raw_clause N))))
-  = mset (map clause N)"
-  by (metis (no_types, lifting) init_clss_init_state map_eq_conv map_map o_def clause_def)
+  "raw_clss_l (raw_init_clss (init_state (map raw_clause N))) = raw_clss_l N"
+  unfolding raw_clss_l_raw_init_clss_conc_init_clss
+  by (metis (full_types) clause_def comp_def init_clss_init_state map_eq_conv map_map)
 
 fun reduce_trail_to where
 "reduce_trail_to M1 S =
@@ -48,7 +51,9 @@ interpretation rough_cdcl: abs_state\<^sub>W_ops
 
     raw_clause "\<lambda>C. TWL_Clause [] C"
     trail "\<lambda>S. hd (raw_trail S)"
-    raw_init_clss raw_learned_clss backtrack_lvl raw_conflicting
+    "(\<lambda>S. raw_init_clss S @ raw_learned_clss S)" backtrack_lvl raw_conflicting
+    conc_learned_clss
+
     cons_trail tl_trail "\<lambda>S. update_conflicting None (add_learned_cls (the (raw_conflicting S)) S)"
     "\<lambda>C. remove_cls (raw_clause C)"
     update_backtrack_lvl
@@ -78,7 +83,9 @@ interpretation rough_cdcl: abs_state\<^sub>W
 
   raw_clause "\<lambda>C. TWL_Clause [] C"
   trail "\<lambda>S. hd (raw_trail S)"
-  raw_init_clss raw_learned_clss backtrack_lvl raw_conflicting
+  "(\<lambda>S. raw_init_clss S @ raw_learned_clss S)" backtrack_lvl raw_conflicting
+  conc_learned_clss
+
   cons_trail tl_trail "\<lambda>S. update_conflicting None (add_learned_cls (the (raw_conflicting S)) S)"
   "\<lambda>C. remove_cls (raw_clause C)"
   update_backtrack_lvl
@@ -94,9 +101,14 @@ proof goal_cases
     apply (rule ext, rename_tac L, case_tac L)
     by (auto simp: abs_state\<^sub>W_ops.mmset_of_mlit.simps[OF stupid_locales] clause_def
     raw_clause_def)
-  have [simp]: "\<And>S. raw_clss_l (restart_learned S) \<subseteq># rough_cdcl.conc_learned_clss S"
+  have [simp]: "\<And>S. raw_clss_l (restart_learned S) \<subseteq># conc_learned_clss S"
     using image_mset_subseteq_mono[OF restart_learned] unfolding mset_map
      by blast
+  have [simp]: "\<And>st C. mset (removeAll (clause C) (map clause (raw_init_clss st))) =
+       removeAll_mset (clause C) (rough_cdcl.conc_init_clss st)"
+    unfolding rough_cdcl.conc_init_clss_def by (metis add.commute add_diff_cancel_left'
+      mset_removeAll union_clss)
+
   have H: "\<And>M2 M1 x1. M2 @ M1 = map mmset_of_mlit x1 \<Longrightarrow>
        map mmset_of_mlit (drop (length x1 - length M1) x1) = M1"
     by (metis add_diff_cancel_right' append_eq_conv_conj drop_map length_append length_map)
@@ -118,7 +130,9 @@ interpretation rough_cdcl: abs_conflict_driven_clause_learning\<^sub>W
 
   raw_clause "\<lambda>C. TWL_Clause [] C"
   trail "\<lambda>S. hd (raw_trail S)"
-  raw_init_clss raw_learned_clss backtrack_lvl raw_conflicting
+  "(\<lambda>S. raw_init_clss S @ raw_learned_clss S)" backtrack_lvl raw_conflicting
+  conc_learned_clss
+
   cons_trail tl_trail "\<lambda>S. update_conflicting None (add_learned_cls (the (raw_conflicting S)) S)"
   "\<lambda>C. remove_cls (raw_clause C)"
   update_backtrack_lvl
@@ -142,7 +156,8 @@ lemma wf_twl_state_cons_trail:
     wf: "wf_twl_state S"
   shows "wf_twl_state (cons_trail L S)"
   using undef wf wf_rewatch[of S ] unfolding wf_twl_state_def Ball_def
-  by (auto simp: cons_trail_def defined_lit_map comp_def image_def twl.raw_clauses_def)
+  by (auto simp: cons_trail_def defined_lit_map comp_def image_def
+    rough_cdcl.conc_clauses_init_learned)
 
 lemma rough_state_of_twl_cons_trail:
   "undefined_lit (raw_trail_twl S) (lit_of L) \<Longrightarrow>
@@ -154,7 +169,8 @@ abbreviation add_init_cls_twl where
 "add_init_cls_twl C S \<equiv> twl_of_rough_state (add_init_cls C (rough_state_of_twl S))"
 
 lemma wf_twl_add_init_cls: "wf_twl_state S \<Longrightarrow> wf_twl_state (add_init_cls L S)"
-  unfolding wf_twl_state_def by (auto simp: wf_watch add_init_cls_def comp_def twl.raw_clauses_def
+  unfolding wf_twl_state_def by (auto simp: wf_watch add_init_cls_def comp_def
+    rough_cdcl.conc_clauses_init_learned
     split: if_split_asm)
 
 lemma rough_state_of_twl_add_init_cls:
@@ -165,7 +181,8 @@ abbreviation add_learned_cls_twl where
 "add_learned_cls_twl C S \<equiv> twl_of_rough_state (add_learned_cls C (rough_state_of_twl S))"
 
 lemma wf_twl_add_learned_cls: "wf_twl_state S \<Longrightarrow> wf_twl_state (add_learned_cls L S)"
-  unfolding wf_twl_state_def by (auto simp: wf_watch add_learned_cls_def twl.raw_clauses_def
+  unfolding wf_twl_state_def by (auto simp: wf_watch add_learned_cls_def
+    rough_cdcl.conc_clauses_init_learned
     split: if_split_asm)
 
 lemma rough_state_of_twl_add_learned_cls:
@@ -179,8 +196,8 @@ lemma set_removeAll_condD: "x \<in> set (removeAll_cond f xs) \<Longrightarrow> 
   by (induction xs) (auto split: if_split_asm)
 
 lemma wf_twl_remove_cls: "wf_twl_state S \<Longrightarrow> wf_twl_state (remove_cls L S)"
-  unfolding wf_twl_state_def by (auto simp: wf_watch remove_cls_def twl.raw_clauses_def comp_def
-    split: if_split_asm dest: set_removeAll_condD)
+  unfolding wf_twl_state_def by (auto simp: wf_watch remove_cls_def
+    comp_def split: if_split_asm dest: set_removeAll_condD)
 
 lemma rough_state_of_twl_remove_cls:
   "rough_state_of_twl (remove_cls_twl L S) = remove_cls L (rough_state_of_twl S)"
@@ -198,7 +215,7 @@ lemma wf_twl_state_wf_twl_state_fold_add_init_cls:
 
 lemma wf_twl_state_epsilon_state[simp]:
   "wf_twl_state (TWL_State [] [] [] 0 None)"
-  by (auto simp: wf_twl_state_def twl.raw_clauses_def)
+  by (auto simp: wf_twl_state_def)
 
 lemma wf_twl_init_state: "wf_twl_state (init_state N)"
   unfolding init_state_def by (auto intro!: wf_twl_state_wf_twl_state_fold_add_init_cls)
@@ -212,7 +229,7 @@ abbreviation tl_trail_twl where
 
 lemma wf_twl_state_tl_trail: "wf_twl_state S \<Longrightarrow> wf_twl_state (tl_trail S)"
   by (auto simp add: twl_of_rough_state_inverse wf_twl_init_state wf_twl_cls_wf_twl_cls_tl
-    tl_trail_def wf_twl_state_def distinct_tl map_tl comp_def twl.raw_clauses_def)
+    tl_trail_def wf_twl_state_def distinct_tl map_tl comp_def)
 
 lemma rough_state_of_twl_tl_trail:
   "rough_state_of_twl (tl_trail_twl S) = tl_trail (rough_state_of_twl S)"
@@ -223,7 +240,7 @@ abbreviation update_backtrack_lvl_twl where
 
 lemma wf_twl_state_update_backtrack_lvl:
   "wf_twl_state S \<Longrightarrow> wf_twl_state (update_backtrack_lvl k S)"
-  unfolding wf_twl_state_def by (auto simp: comp_def twl.raw_clauses_def)
+  unfolding wf_twl_state_def by (auto simp: comp_def)
 
 lemma rough_state_of_twl_update_backtrack_lvl:
   "rough_state_of_twl (update_backtrack_lvl_twl k S) = update_backtrack_lvl k
@@ -237,7 +254,7 @@ abbreviation update_conflicting_twl where
 
 lemma wf_twl_state_update_conflicting:
   "wf_twl_state S \<Longrightarrow> wf_twl_state (update_conflicting k S)"
-  unfolding wf_twl_state_def by (auto simp: comp_def twl.raw_clauses_def)
+  unfolding wf_twl_state_def by (auto simp: comp_def)
 
 lemma rough_state_of_twl_update_add_learned_cls:
   "rough_state_of_twl (update_conflicting_twl None (add_learned_cls_twl C S)) =
@@ -261,7 +278,7 @@ lemma rough_state_of_twl_update_conflicting:
   using rough_state_of_twl twl_of_rough_state_inverse wf_twl_state_update_conflicting by fast
 
 abbreviation raw_clauses_twl where
-"raw_clauses_twl S \<equiv> twl.raw_clauses (rough_state_of_twl S)"
+"raw_clauses_twl S \<equiv> raw_clauses (rough_state_of_twl S)"
 
 abbreviation restart_twl where
 "restart_twl S \<equiv> twl_of_rough_state (restart' (rough_state_of_twl S))"
@@ -275,7 +292,7 @@ lemma wf_wf_restart': "wf_twl_state S \<Longrightarrow> wf_twl_state (restart' S
    apply (rename_tac x)
    apply (subgoal_tac "wf_twl_cls (raw_trail S) x")
     apply (case_tac x)
-  using restart_learned by (auto simp: twl.raw_clauses_def comp_def dest: mset_union_mset_setD)
+  using restart_learned by (auto simp: comp_def dest: mset_union_mset_setD)
 
 lemma rough_state_of_twl_restart_twl:
   "rough_state_of_twl (restart_twl S) = restart' (rough_state_of_twl S)"
@@ -298,13 +315,13 @@ proof -
     by auto
   have [simp]: "no_dup (drop (length M - length M1) M)"
     using n_d by (metis distinct_drop drop_map)
-  have "\<And>C. C \<in> set (twl.raw_clauses S) \<Longrightarrow> wf_twl_cls (raw_trail S) C"
+  have "\<And>C. C \<in> set (raw_clauses S) \<Longrightarrow> wf_twl_cls (raw_trail S) C"
     using wf by (auto simp: S comp_def wf_twl_state_def)
   then show ?thesis
     unfolding wf_twl_state_def S
     using wf_twl_cls_append[of "take (length M - length M1) M" "drop (length M - length M1) M",
       unfolded M[symmetric]]
-    by (simp_all add: n_d twl.raw_clauses_def)
+    by (simp_all add: n_d)
 qed
 
 lemma trail_twl_twl_rough_state_reduce_trail_to:
@@ -361,7 +378,8 @@ proof -
     by (auto simp add: assms)
   moreover have "trail_twl (twl_of_rough_state (reduce_trail_to M1 (rough_state_of_twl st))) = M1"
     using trail_twl_twl_rough_state_reduce_trail_to[OF assms(1)] .
-  ultimately show ?st using S unfolding rough_cdcl.state_def by auto
+  ultimately show ?st using S unfolding rough_cdcl.state_def
+    by (metis (no_types) prod.inject twl2.raw_clss_l_raw_init_clss_conc_init_clss)
 qed
 
 lemma add_learned_cls_rough_state_of_twl_simp:
@@ -370,12 +388,12 @@ lemma add_learned_cls_rough_state_of_twl_simp:
     "trail (add_learned_cls z (rough_state_of_twl st)) = trail_twl st"
     "rough_cdcl.conc_init_clss (add_learned_cls z (rough_state_of_twl st)) =
       rough_cdcl.conc_init_clss (rough_state_of_twl st)"
-    "rough_cdcl.conc_learned_clss (local.add_learned_cls z (rough_state_of_twl st)) =
-      {#mset z#} + rough_cdcl.conc_learned_clss (rough_state_of_twl st)"
+    "conc_learned_clss (local.add_learned_cls z (rough_state_of_twl st)) =
+      {#mset z#} + conc_learned_clss (rough_state_of_twl st)"
     "backtrack_lvl (add_learned_cls z (rough_state_of_twl st)) = backtrack_lvl_twl st"
   using assms wf_twl_state_rough_state_of_twl[of st]
   unfolding wf_twl_state_def apply
-  (auto simp: wf_watch add_learned_cls_def comp_def twl.raw_clauses_def local.clause_watch
+  (auto simp: wf_watch add_learned_cls_def comp_def local.clause_watch
     ac_simps
     split: if_split_asm)
   done
@@ -389,10 +407,11 @@ sublocale wf_twl: abs_state\<^sub>W_ops
 
   "\<lambda>C. raw_clause C" "\<lambda>C. TWL_Clause [] C"
   trail_twl "\<lambda>S. hd (raw_trail_twl S)"
-  raw_init_clss_twl
-  raw_learned_clss_twl
+  raw_clauses_twl
   backtrack_lvl_twl
   raw_conflicting_twl
+  conc_learned_clss_twl
+
   cons_trail_twl
   tl_trail_twl
   "\<lambda>S. update_conflicting_twl None (add_learned_cls_twl (the (raw_conflicting_twl S)) S)"
@@ -405,6 +424,10 @@ sublocale wf_twl: abs_state\<^sub>W_ops
   restart_twl
   by unfold_locales
 
+lemma wf_twl_conc_init_clss_restart_twl[simp]:
+  "wf_twl.conc_init_clss (restart_twl S) = wf_twl.conc_init_clss S"
+  using rough_state_of_twl_restart_twl wf_twl.conc_init_clss_def by auto
+
 sublocale wf_twl: abs_state\<^sub>W
   clause
   raw_clss_l "op @"
@@ -414,10 +437,11 @@ sublocale wf_twl: abs_state\<^sub>W
 
   "\<lambda>C. raw_clause C" "\<lambda>C. TWL_Clause [] C"
   trail_twl "\<lambda>S. hd (raw_trail_twl S)"
-  raw_init_clss_twl
-  raw_learned_clss_twl
+  raw_clauses_twl
   backtrack_lvl_twl
   raw_conflicting_twl
+  conc_learned_clss_twl
+
   cons_trail_twl
   tl_trail_twl
   "\<lambda>S. update_conflicting_twl None (add_learned_cls_twl (the (raw_conflicting_twl S)) S)"
@@ -438,7 +462,7 @@ proof goal_cases
     apply (rule ext, rename_tac L, case_tac L)
     by (auto simp: abs_state\<^sub>W_ops.mmset_of_mlit.simps[OF stupid_locales] clause_def
     raw_clause_def)
-  have [simp]: "\<And>S. raw_clss_l (restart_learned S) \<subseteq># rough_cdcl.conc_learned_clss S"
+  have [simp]: "\<And>S. raw_clss_l (restart_learned S) \<subseteq># conc_learned_clss S"
     using image_mset_subseteq_mono[OF restart_learned] unfolding mset_map
      by blast
   interpret abs_state\<^sub>W_ops  clause
@@ -449,11 +473,10 @@ proof goal_cases
 
     "\<lambda>C. raw_clause C" "\<lambda>C. TWL_Clause [] C"
     by unfold_locales
-  have abs: "\<And>S. abs_state\<^sub>W_ops.state raw_clss_l mset trail_twl raw_init_clss_twl
-    raw_learned_clss_twl backtrack_lvl_twl raw_conflicting_twl S =
+  have abs: "\<And>S. abs_state\<^sub>W_ops.state raw_clss_l mset trail_twl raw_clauses_twl
+    backtrack_lvl_twl raw_conflicting_twl conc_learned_clss_twl S =
     rough_cdcl.state (rough_state_of_twl S)"
-    unfolding abs_state\<^sub>W_ops.state_def[OF stupid_locales] ..
-
+    using wf_twl.conc_init_clss_def unfolding abs_state\<^sub>W_ops.state_def[OF stupid_locales] by auto
   show ?case
      apply unfold_locales
                using rough_cdcl.hd_raw_conc_trail unfolding ugly apply blast
@@ -473,11 +496,12 @@ proof goal_cases
            rough_state_of_twl_update_conflicting abs; fail)[]
      using twl_of_rough_state_reduce_trail_to(1) unfolding abs
      using rough_cdcl.conc_init_clss_restart_state rough_cdcl.conc_learned_clss_restart_state
-     apply (simp add: rough_cdcl.resolve_conflicting twl2.rough_state_of_twl_update_conflicting)
+     apply (simp add: rough_cdcl.resolve_conflicting twl2.rough_state_of_twl_update_conflicting;
+       fail)
   using twl_of_rough_state_reduce_trail_to(1) unfolding abs
   using rough_cdcl.conc_init_clss_restart_state rough_cdcl.conc_learned_clss_restart_state
   by (auto simp: rough_state_of_twl_restart_twl abs
-    rough_cdcl.state_def rough_state_of_twl_init_state comp_def)[7]
+    rough_cdcl.state_def rough_state_of_twl_init_state comp_def)[8]
   qed
 
 
@@ -490,10 +514,11 @@ sublocale wf_twl: abs_conflict_driven_clause_learning\<^sub>W
 
   "\<lambda>C. raw_clause C" "\<lambda>C. TWL_Clause [] C"
   trail_twl "\<lambda>S. hd (raw_trail_twl S)"
-  raw_init_clss_twl
-  raw_learned_clss_twl
+  raw_clauses_twl
   backtrack_lvl_twl
   raw_conflicting_twl
+  conc_learned_clss_twl
+
   cons_trail_twl
   tl_trail_twl
   "\<lambda>S. update_conflicting_twl None (add_learned_cls_twl (the (raw_conflicting_twl S)) S)"
@@ -521,6 +546,16 @@ propagate_twl_rule: "(L, C) \<in> candidates_propagate_twl S \<Longrightarrow>
   raw_conflicting_twl S = None \<Longrightarrow>
   propagate_twl S S'"
 
+lemma cdcl\<^sub>W_all_struct_inv_clause_distinct_mset:
+  "cdcl\<^sub>W_mset.cdcl\<^sub>W_all_struct_inv (wf_twl.state S) \<Longrightarrow>
+    C \<in> set (CDCL_Two_Watched_Literals.raw_clauses_twl S) \<Longrightarrow> distinct (raw_clause C)"
+  unfolding cdcl\<^sub>W_mset.cdcl\<^sub>W_all_struct_inv_def cdcl\<^sub>W_mset.distinct_cdcl\<^sub>W_state_def
+     distinct_mset_set_def wf_twl.conc_clauses_init_learned
+  by (metis distinct_mset_distinct in_clss_mset_clss in_clss_union_clss
+    rough_cdcl.conc_init_clss_def twl2.raw_clss_l_raw_init_clss_conc_init_clss
+    wf_twl.conc_init_clss_def wf_twl.init_clss_state_conc_init_clss
+    wf_twl.learned_clss_state_conc_learned_clss wf_twl.mset_ccls_ccls_of_cls)
+
 inductive_cases propagate_twlE: "propagate_twl S T"
 lemma propagate_twl_iff_propagate:
   assumes inv: "cdcl\<^sub>W_mset.cdcl\<^sub>W_all_struct_inv (wf_twl.state S)"
@@ -529,24 +564,22 @@ proof
   assume ?P
   then obtain L E where
     "raw_conflicting_twl S = None" and
-    CL_Clauses: "E \<in> set (wf_twl.raw_clauses S)" and
+    CL_Clauses: "E \<in> set (raw_clauses_twl S)" and
     LE: "L \<in># clause E" and
     tr_CNot: "trail_twl S \<Turnstile>as CNot (remove1_mset L (clause E))" and
     undef_lot[simp]: "undefined_lit (trail_twl S) L" and
     "T \<sim> cons_trail_twl (Propagated L E) S"
     by (blast elim: wf_twl.propagate_absE)
   have "distinct (raw_clause E)"
-    using inv CL_Clauses unfolding cdcl\<^sub>W_mset.cdcl\<^sub>W_all_struct_inv_def distinct_mset_set_def
-    cdcl\<^sub>W_mset.distinct_cdcl\<^sub>W_state_def wf_twl.raw_clauses_def by (auto simp: clause_def)
+    using inv CL_Clauses cdcl\<^sub>W_all_struct_inv_clause_distinct_mset by blast
   then have X: "remove1_mset L (mset (raw_clause E)) = mset_set (set (raw_clause E) - {L})"
     by (auto simp: multiset_eq_iff raw_clause_def count_mset distinct_filter_eq_if)
   have "(L, E) \<in> candidates_propagate_twl S"
     apply (rule wf_candidates_propagate_complete)
-         using rough_state_of_twl apply auto[]
-        using CL_Clauses unfolding wf_twl.raw_clauses_def twl.raw_clauses_def
-        apply auto[]
-       using LE apply (simp add: clause_def)
-      using tr_CNot X apply (simp add: clause_def)
+         using rough_state_of_twl apply (auto; fail)[]
+        using CL_Clauses apply (auto; fail)[]
+       using LE apply (simp add: clause_def; fail)
+      using tr_CNot X apply (simp add: clause_def; fail)
      using undef_lot apply blast
      done
   show ?T
@@ -566,22 +599,22 @@ next
     C'S: "C \<in> set (raw_clauses_twl S)" and
     L: "set (watched C) - uminus ` lits_of_l (trail_twl S) = {L}" and
     undef: "undefined_lit (trail_twl S) L"
-    using LC unfolding candidates_propagate_def wf_twl.raw_clauses_def by auto
+    using LC unfolding candidates_propagate_def by auto
   have dist: "distinct (raw_clause C)"
-    using inv C'S unfolding cdcl\<^sub>W_mset.cdcl\<^sub>W_all_struct_inv_def cdcl\<^sub>W_mset.distinct_cdcl\<^sub>W_state_def
-     distinct_mset_set_def twl.raw_clauses_def by (fastforce simp: clause_def)
+    using inv C'S cdcl\<^sub>W_all_struct_inv_clause_distinct_mset by blast
   then have C_L_L: "mset_set (set (raw_clause C) - {L}) = clause C - {#L#}"
     by (metis distinct_mset_distinct distinct_mset_minus distinct_mset_set_mset_ident mset_remove1
       set_mset_mset set_remove1_eq clause_def)
 
   show ?P
     apply (rule wf_twl.propagate_abs_rule[of S C L])
-        using confl apply auto[]
-       using C'S unfolding twl.raw_clauses_def apply (simp add: wf_twl.raw_clauses_def)
-       using L unfolding candidates_propagate_def apply (auto simp: raw_clause_def clause_def)[]
+        using confl apply (auto; fail)[]
+       using C'S apply (simp; fail)
+       using L unfolding candidates_propagate_def
+       apply (auto simp: raw_clause_def clause_def; fail)[]
       using wf_candidates_propagate_sound[OF _ LC] rough_state_of_twl dist
-      apply (simp add: distinct_mset_remove1_All true_annots_true_cls clause_def)
-     using undef apply simp
+      apply (simp add: distinct_mset_remove1_All true_annots_true_cls clause_def; fail)
+     using undef apply (simp; fail)
     using T undef unfolding cdcl\<^sub>W_mset.state_eq_def by auto
 qed
 
@@ -602,7 +635,7 @@ proof
   assume ?C
   then obtain D where
     S: "raw_conflicting_twl S = None" and
-    D: "D \<in> set (wf_twl.raw_clauses S)" and
+    D: "D \<in> set (raw_clauses_twl S)" and
     MD: "trail_twl S \<Turnstile>as CNot (clause D)" and
     T: "T \<sim> update_conflicting_twl (Some (raw_clause D)) S"
     by (elim wf_twl.conflict_absE)
@@ -610,7 +643,7 @@ proof
   have "D \<in> candidates_conflict_twl S"
     apply (rule wf_candidates_conflict_complete)
        apply simp
-      using D apply (auto simp: wf_twl.raw_clauses_def twl.raw_clauses_def)[]
+      using D apply (auto; fail)[]
     using MD S by auto
   moreover have "T \<sim> twl_of_rough_state (update_conflicting (Some (raw_clause D))
   (rough_state_of_twl S))"
@@ -625,8 +658,8 @@ next
     confl: "raw_conflicting_twl S = None"
     by (auto elim: conflict_twlE)
   have
-    "C \<in> set (wf_twl.raw_clauses S)"
-    using C unfolding candidates_conflict_def wf_twl.raw_clauses_def twl.raw_clauses_def by auto
+    "C \<in> set (raw_clauses_twl S)"
+    using C unfolding candidates_conflict_def by auto
  moreover have "trail_twl S \<Turnstile>as CNot (clause C)"
     using wf_candidates_conflict_sound[OF _ C] by auto
  ultimately show ?C apply -
